\subsection{1. formula (higher derivation of 
      \(\hat{\mathbb{D}}\left( \xi_k \begin{matrix} 
      P_m \\ \Omega_m \end{matrix} \bigg| x  \right)\))}
      
\begin{definition}
      Let us have an O  operator
      
      \begin{align}
            \biigO_{t = 1}^m g(f(t) \ o \  \lambda) :=
            g(f(1) \ o \  g(f(2) \ o \   g(... g(f(m) )...)))
      \end{align}
      
      where o is some binary arithmetic operation. 
      We will \(f(t)\) call as nucleus, \(\lambda\) 
      as the tail, and g(.) as surface. The tail is 
      where the operator will iterate.
\end{definition}

\begin{definition}
      \(\mathcal{T}\) function is recursive \(\mathcal{T}(n_1, 
      n_2, ..., n_k | x) = n_1^{\mathcal{T}(n_2, ..., n_k | x)}\) 
      with endpoints \(\mathcal{T}(n_k | x ) = n_k^x\) , 
      where the coefficients  \((n_1, n_2, ..., n_k)\) make up the
      \(\xi\) vector,
      when it applies \(n_1, n_2, ..., n_k \in  \mathbb{C}\).  
      \(\mathcal{T}(n_1, n_2, ..., n_k | x) \) is the \(\mathcal{T
      }\) k-th order function with base \(x\).
\end{definition}

\begin{definition}
      Let us have function

      \begin{align}
            \mathcal{T}(\xi_k |x) + \frac{(x-t_1)(x-t_2)...
            (x-t_n)}{(x-s_1)(x-s_2)...(x-s_m)} \equiv 
            \mathbb{D}\left( \xi_k \begin{matrix} \iota_n
            \\ \zeta_m \end{matrix} \bigg| x \right)=w
      \end{align}

      where \(\bigotimes_{u=1}^n t_u = \iota_n; 
      \bigotimes_{r=1}^m s_r = \zeta_m\)
      then its inversion can be written in the form

      \begin{align}
            x = \mathbb{T}\left( \xi_k \begin{matrix} \iota_n 
            \\ \zeta_m \end{matrix} \bigg| w \right)
      \end{align}

\end{definition}

\begin{align}
      \left[\hat{\mathbb{D}}\left( \xi_k \begin{matrix} P_m \\ 
      \Omega_m \end{matrix} \bigg| x  \right)\right]^{(\xi)} &= 
      \frac{d^\xi}{dx^\xi}(\mathcal{T}(\bigotimes_{m \geq t \geq 
      n}x_t | x) ) + \frac{d^\xi}{dx^\xi}\left(\prod_{i=1}^m(x -
      \omega_i)^{p_i}^{v}  \right)\\
      & = \mathcal{T}(\bigotimes_{m \geq t \geq n}x_t| x) \ln^\xi 
      (x_m) \biigO_{\lambda = 1}^{m-1} \left[\sum_{u_{\lambda}=1}^{u_{
      \lambda-1}}\ln^{u_{\lambda}}(x_{m-\lambda}) \mathcal{T}(
      \bigotimes_{q = \lambda-1}^\lambda x_{m-q} |x)^{u_{\lambda
      }} \right] + \\
      & + \xi! \sum_{\sum_{j=1}^m k_j = \xi}\prod_{1 \leq t \leq 
      m} \frac{(x - \omega_t)^{p_k v}\Gamma(1+p_t v)}{k_t\Gamma(
      1+p_t v - k_t)}
\end{align}

then 

\begin{align}
      \hat{\mathbb{T}}^{(\xi)}\left( \xi_k \begin{matrix} P_m
      \\ \Omega_m \end{matrix} \bigg| x  \right) = \sum \frac{(-1)^{
      \beta_1 + \xi}(\beta_1 -1)!}{\prod_{i=2}^\xi (\beta_i)!i!^{
      \beta_i}} \hat{\mathbb{D}}^{(1)}\left( \xi_k \begin{matrix}
      P_m \\ \Omega_m \end{matrix} \bigg| x  \right) \prod_{j=2}^\xi
      \left(\hat{\mathbb{D}}^{(i)}\left( \xi_k \begin{matrix} P_m \\
      \Omega_m \end{matrix} \bigg| x  \right)^{\beta_i}\right)
\end{align}

where

\begin{align}
      \beta_1 \leq 2n-1,  \beta_i \geq 0,  \sum_{i=2}^n 
      \beta_i = \beta_1 - n,   \sum_{i=2}^n i \beta_i = \beta_1 - 1
\end{align}

Hence

\begin{align}
      \hat{\mathbb{T}}^{(\xi)}\left( \xi_k \begin{matrix} P_m \\
      \Omega_m \end{matrix} \bigg| x  \right) &= \sum \frac{(-1)^{
      \beta_1 + \xi}(\beta_1 -1)!}{\prod_{i=2}^\xi (\beta_i)!i!^{\beta_i
      }} (\prod_{\lambda = 1}^k (\ln(n_\lambda) \mathcal{T}(\bigotimes_{
      j=1}^\lambda n_j |x) + \\
      &+\sum_{i=1}^m p_i \prod_{j=1}^m (x-\omega_j)^{p_i-\delta_{i, 
      j}(1)} )\prod_{j=2}^\xi \left(\hat{\mathbb{D}}^{(i)}\left( \xi_k
      \begin{matrix} P_m \\ \Omega_m \end{matrix} \bigg| x  \right)^{
      \beta_i}\right)\\
      &= \sum \frac{(-1)^{\beta_1 + \xi}(\beta_1 -1)!}{\prod_{i=2}^\xi
      (\beta_i)!i!^{\beta_i}} (\prod_{\lambda = 1}^k (\ln(n_\lambda) 
      \mathcal{T}(\bigotimes_{j=1}^\lambda n_j |x) + \\
      &+\sum_{i=1}^m p_i \prod_{j=1}^m (x-\omega_j)^{p_i-\delta_{i, 
      j}(1)} )\prod_{j=2}^\xi \left(\mathcal{T}(\bigotimes_{m \geq t 
      \geq n}x_t| x) \ln^i (x_m) \right.\\
      &\left. \biigO_{\lambda = 1}^{m-1} \left[\sum_{u_{\lambda}=1}^{
      u_{\lambda-1}}\ln^{u_{\lambda}}(x_{m-\lambda}) \mathcal{T}(
      \bigotimes_{q = \lambda-1}^\lambda x_{m-q} |x)^{u_{\lambda}} 
      \right] + \right.\\
      &\left.+ i! \sum_{\sum_{j=1}^m k_j = i}\prod_{1 \leq t \leq
      m} \frac{(x - \omega_t)^{p_k v}\Gamma(1+p_t v)}{k_t\Gamma(1+
      p_t v - k_t)}\right)^{\beta_i}
\end{align}
