\subsection{9. Formule (Explicit representation of the nested power tower function)}

\begin{align}
        \mathcal{T}\left(\bigotimes_{n=1}^ka_n | x\right) =
        \sum_{n=0}^\infty \frac{1}{n!}\left(\biigO_{l=1}^{k-1}
        \ln(a_l)\left[\sum_{n_l\geq0}\frac{1}{n_l!}\left(
        \lambda_l\right)^{n_l}\right]^{\Lambda(l, k, \ln(a_k)x}\right)^n
\end{align}

where \(\Lambda(l, k, \ln(a_k)x) :=\left[\lceil tanh^2(l-k+1)
\rceil+\delta_{l, k-1}(\ln(a_k)x)\right]\), this function is 
equal to \(\ln(a_k)x\) iff \(l=k-1\), in other cases, its 0.
Then higher derivation of this function is

\begin{align}
        \frac{d^\xi\mathcal{T}}{dx^\xi}\left(\bigotimes_{n=1}^ka_n
        | x\right) = \sum_{n\geq0}\frac{1}{n!}\ln^n(a_1)
        \frac{d^\xi}{dx^\xi}\left(\sum_{n_1\geq0}\frac{1}{n_1!}g(x)\right)
\end{align}

We use the Multinomial formula for

\begin{align}
        \frac{d^\xi}{dx^\xi}\left(\sum_{n_1\geq0}\frac{1}{
        n_1!}g(x)\right) &=  \frac{d^\xi}{dx^\xi} \sum_{n_1
        \geq0} \left(\sum_{\substack{0\leq r_1 \leq...\leqr_n
        \leq n_1 \\ r_1 +...+r_n = n_1}}\prod_{i=1}^n \frac{1}{
        r_i}\right)g^{n_1}(x) \\
        &=\sum_{n_1\geq0} \left(\sum_{\substack{0\leq r_1 \leq.
        ..\leqr_n\leq n_1 \\ r_1 +...+r_n = n_1}}\prod_{i=1}^n 
        \frac{1}{r_i}\right)\frac{d^\xi}{dx^\xi}g^{n_1}(x)
\end{align}

There is set \(S=\{r_1, ..., r_n\}\) of many distinct elements 
with \(m \leq n\), call these distinct elements \(s_1, ..., s_m\).
And define \(N(s_i) = \# \mbox{of} \ s_i \ \mbox{appears in} \ 
(r_1, ..., r_n) \), then we see that the number of time \(a_{r_1}
...a_{r_n}\) is is counted is equal to 

\begin{align}
        \frac{n!}{N(s_1)!...N(s_m)!}
\end{align}

thus we have

\begin{align}
        \sum_{n_1\geq0} \left(\sum_{\substack{0\leq
        r_1 \leq...\leqr_n\leq n_1 \\ r_1 +...+r_n =
        n_1}}\frac{n!}{N(s_1)!...N(s_m)!}\prod_{i=1}^n
        \frac{1}{r_i}\right)\frac{d^\xi}{dx^\xi}g^{n_1}(x)
\end{align}

hence

\begin{align}
        \frac{d^\xi}{dx^\xi}\left(\sum_{n_1\geq0}\frac{1}{
        n_1!}g(x)\right) &=\sum_{n\geq0}\frac{1}{n!}\ln^n(
        a_1) \frac{d^\xi}{dx^\xi}\left(\sum_{n_1\geq0}\frac{1}{
        n_1!}g(x)\right) \\
        &=\sum_{n\geq 0}\frac{1}{n!}\ln^n(a_1)\sum_{n_1\geq0}
        \left(\sum_{\substack{0\leq r_1 \leq...\leqr_n\leq n_1 
        \\ r_1 +...+r_n = n_1}}\prod_{i=1}^n \frac{1}{r_i}\right)
        \frac{d^\xi}{dx^\xi}g^{n_1}(x) \\
        & =\sum_{n_0\geq 0}\frac{1}{n_0!}\biigO_{l=1}^{k-1}
        \ln^{n_{l-1}}(a_l)
        \sum_{n_l\geq0} \left(\sum_{\substack{0\leq r_1 \leq...
        \leqr_n\leq n_l \\ r_1 +...+r_n = n_l}}\frac{n_{l-1}!}{
        N(s_1)!...N(s_m)!}\prod_{i=1}^{n_{l-1}} \frac{1}{r_i}
        \right)(\lambda_l)^{n_l \Lambda(l, k,\frac{\ln(a_k)x^{
        -\xi+n_{l-1}}}{((1-\xi + n_{l-1})_\xi)^{-1}}}
\end{align}

then we use equation \ref{w}, so we get

\begin{align}
        \mathcal{T}(\bigotimes_{k \geq t \geq 1}a_t| x) 
        \ln^\xi (a_k) \biigO_{\lambda = 1}^{m-1} R\left[
        \sum_{u_{\lambda}=1}^{u_{\lambda-1}}\ln^{u_{
        \lambda}}(a_{k-\lambda}) \mathcal{T}(\bigotimes_{
        q = \lambda-1}^\lambda a_{k-q} |x)^{u_{\lambda}} 
        \right] = \\=\sum_{n_0\geq 0}\frac{1}{n_0!}\biigO_{l=1}^{k-1}
        \ln^{n_{l-1}}(a_l)
        \sum_{n_l\geq0} \left(\sum_{\substack{0\leq r_1 
        \leq...\leqr_n\leq n_l \\ r_1 +...+r_n = n_l}}
        \frac{n_{l-1}!}{N(s_1)!...N(s_m)!}\prod_{i=1}^{n_{l-1}}
        \frac{1}{r_i}\right)(\lambda_l)^{n_l \Lambda(l, k,\frac{
        \ln(a_k)x^{-\xi+n_{l-1}}}{((1-\xi + n_{l-1})_\xi)^{-1}}}
\end{align}

we solve this equation for \( \mathcal{T}(\bigotimes_{k 
\geq t \geq 1}a_t| x)\)

\begin{align}
        \mathcal{T}(\bigotimes_{k \geq t \geq 1}a_t| x)
        &=\left(\ln^\xi (a_k) \biigO_{\lambda = 1}^{m-1} 
        \left[ \lceil \tanh^2(\lambda -1)\rceil+\delta_{\lambda,
        1}(S_2((u_1, \xi))\right]\left[\sum_{u_{\lambda}=1}^{
        u_{\lambda-1}}\ln^{u_{\lambda}}(a_{k-\lambda}) \mathcal{
        T}(\bigotimes_{q = \lambda-1}^\lambda a_{k-q} |x)^{u_{
        \lambda}} \right]\right)^{-1}\times \\ &\times \sum_{
        n_0\geq 0}\frac{1}{n_0!}\biigO_{l=1}^{k-1}
        \ln^{n_{l-1}}(a_l)
        \sum_{n_l\geq0} \left(\sum_{\substack{0\leq r_1 \leq..
        .\leq r_n\leq n_l \\ r_1 +...+r_n = n_l}}\frac{n_{l-1}!
        }{N(s_1)!...N(s_m)!}\prod_{i=1}^{n_{l-1}} \frac{1}{r_i}
        \right)(\lambda_l)^{n_l \Lambda(l, k,\frac{\ln(a_k)x^{
        -\xi+n_{l-1}}}{((1-\xi + n_{l-1})_\xi)^{-1}}}
\end{align}
