\subsection{10. Formule (The explicit formula for Fibonacci sequence)}

\begin{align}
      _\lambda \rho_n^{n+1} = \sum_{i=0}^n \rho^i
\end{align}

where \(1 \leq \lambda n+1\), 
\(\lambda \in \mathbb{Z}^+\).
then

\begin{align}
      _\lambda\rho_n^{n+2} &= \sum_{n=1}^{n+1}_\lambda\rho_n^i 
      = \sum_{i=1}^n  _\lambda\rho_n^i + \sum_{i=0}^n _\lambda\rho_n^i \\
      _\lambda\rho_n^{n+3} &= \sum_{i=2}^n_\lambda\rho_n^i + 
      \sum_{i=1}^n_\lambda\rho_n^i + 2\sum_{i=0}^n_\lambda\rho_n^i \\
\end{align}

We establish hypothesis 

\begin{align}
      _\lambda\rho_n^{n+m}= \sum_{k=0}^m F_{k+1}\sum_{i=m-k}^n 
      _\lambda\rho_n^{i}=\sum_{k=0}^m F_{k+1}\left( \frac{_\lambda
      \rho_n^{n+1} - _\lambda\rho_n^{m-k}}{_\lambda\rho_n - 1}\right)
\end{align}

Our goal is to found the explicit formula for Fibonacci sequence.

\begin{align}
      \begin{pmatrix}
            _1\rho_n^n \\
            _2\rho_n^n \\
            \vdots\\
            _n\rho_n^n \\
      \end{pmatrix}
      =
      \begin{pmatrix}
            \frac{1}{_1\rho_n^m}\sum_{k=0}^m 
            F_{k+1}\left( \frac{_1\rho_n^{n+1} -
            _1\rho_n^{m-k}}{_1\rho_n - 1}\right) \\
            \frac{1}{_2\rho_n^m}\sum_{k=0}^m F_{k+1}
            \left( \frac{_2\rho_n^{n+1} - _2\rho_n^{
            m-k}}{_1\rho_n - 1}\right) \\
            \vdots \\
            \frac{1}{_n\rho_n^m}\sum_{k=0}^m F_{k+1}\left(
            \frac{_n\rho_n^{n+1} - _n\rho_n^{m-k}}{_m\rho_n
            - 1}\right) \\
      \end{pmatrix}
\end{align}

\begin{theorem}
      \((\forall \xi)(\forall \lambda)(\xi 
      \geq 1)(1 \leq \lambda \leq n+1),\) then
      
      \begin{align}
            F_{\xi+1}=\left(\frac{_\lambda \rho_n^{n+1}-_\lambda
            \rho_n^{\Lambda(\xi)-\xi}}{_\lambda \rho_n-1}\right)
                  \sum_{k=1}^{\Lambda(\xi)}\frac{\mu(k)_\lambda\rho_n^2
            }{_\lambda\rho_n^{-\frac{\Lambda(\xi)}{k}}}
      \end{align}
      
      where \(\mu(k)\) is MÃ¶bius function
      
      \begin{align}
            \Lambda(\xi) \cong e \exp{\left(W\left(
            \frac{1}{e}\ln\left(\frac{\xi!}{\sqrt{2
            \pi}}\right)\right)\right)}+\frac{1}{2}
      \end{align}
\end{theorem}
